spot/GC.SPOT.ConcreteFull.fst
@@ -13,11 +13,14 @@ module ThreeObjects = GC.SPOT.ThreeObjects
 module ConcreteMinor = GC.SPOT.ConcreteMinor
 module ConcreteMajor = GC.SPOT.ConcreteMajor
 module ConcreteScenarios = GC.SPOT.ConcreteScenarios
+module ConcreteForwarding = GC.SPOT.ConcreteForwarding
 module Postconditions = GC.SPOT.Postconditions
 module Preconditions = GC.SPOT.Preconditions
 module SpecHeap = GC.Spec.Heap
 module SpecObj = GC.Spec.Object
 module SpecFields = GC.Spec.Fields
+module SpecMark = GC.Spec.Mark
+module SpecMarkBoundedInv = GC.Spec.MarkBoundedInv
 module SpecCorrectness = GC.Spec.Correctness
 module HeapGraph = GC.Spec.HeapGraph
 module HeapModel = GC.Spec.HeapModel
@@ -31,10 +34,24 @@ module CheneyBFS = GC.Gen.CheneyBFS
 module GenImpl = GC.Gen.Impl
 module MinorFwd = GC.Gen.MinorCollectForwarding
 module MCFH = GC.Gen.MinorCollectForwarding.Helpers
+module MajorGC = GC.Impl
+module MarkBoundedImpl = GC.Impl.MarkBounded
+
+let roots_match_u64_mem_in_stack
+  (roots: seq U64.t) (st: seq obj_addr) (r: U64.t)
+  : Lemma
+      (requires GenImpl.roots_match_stack roots st /\ Seq.mem r roots)
+      (ensures is_val_addr r /\ Seq.mem (r <: obj_addr) st)
+  =
+  GenImpl.roots_match_stack_root_is_val_addr roots st r;
+  GC.Spec.Base.is_val_addr_spec r;
+  let r_obj = (r <: obj_addr) in
+  assert ((r_obj <: U64.t) == r);
+  GenImpl.roots_match_stack_root_in_stack roots st r_obj
 
 let post_roots_mem_c
   (r: unit{ConcreteMajor.spot_major_room})
-  (roots_out: seq U64.t) (st: seq obj_addr)
+  (roots_out: seq U64.t) (st: seq obj_addr) (cap: nat)
   : Lemma
       (requires
         GenImpl.gen_gc_roots_post
@@ -42,8 +59,16 @@ let post_roots_mem_c
           (ConcreteMajor.spot_major_heap r)
           (ConcreteMajor.spot_major_fp r)
           (ThreeObjects.spot_roots (ConcreteMajor.spot_c r))
-          roots_out st)
-      (ensures Seq.mem (ConcreteMajor.spot_c r <: U64.t) roots_out)
+          roots_out st cap)
+      (ensures
+        Seq.mem (ConcreteMajor.spot_c r <: U64.t) roots_out /\
+        Seq.mem (ConcreteMajor.spot_c r)
+          (GenImpl.gen_gc_prepared_roots
+            ConcreteMinor.spot_minor2
+            (ConcreteMajor.spot_major_heap r)
+            (ConcreteMajor.spot_major_fp r)
+            (ThreeObjects.spot_roots (ConcreteMajor.spot_c r))
+            st cap))
   =
   let c = ConcreteMajor.spot_c r in
   let roots = ThreeObjects.spot_roots c in
@@ -69,23 +94,18 @@ let post_roots_mem_c
   assert (Seq.length roots_out > 0);
   assert (Seq.index roots_out 0 == (c <: U64.t));
   FStar.Seq.Properties.seq_mem_k roots_out 0;
-  assert (Seq.mem (c <: U64.t) roots_out)
-
-let roots_match_u64_mem_in_stack
-  (roots: seq U64.t) (st: seq obj_addr) (r: U64.t)
-  : Lemma
-      (requires GenImpl.roots_match_stack roots st /\ Seq.mem r roots)
-      (ensures is_val_addr r /\ Seq.mem (r <: obj_addr) st)
-  =
-  GenImpl.roots_match_stack_root_is_val_addr roots st r;
-  GC.Spec.Base.is_val_addr_spec r;
-  let r_obj = (r <: obj_addr) in
-  assert ((r_obj <: U64.t) == r);
-  GenImpl.roots_match_stack_root_in_stack roots st r_obj
+  assert (Seq.mem (c <: U64.t) roots_out);
+  let prepared_roots = GenImpl.gen_gc_prepared_roots
+    ConcreteMinor.spot_minor2
+    (ConcreteMajor.spot_major_heap r)
+    (ConcreteMajor.spot_major_fp r)
+    roots st cap in
+  assert (GenImpl.roots_match_stack roots_out prepared_roots);
+  roots_match_u64_mem_in_stack roots_out prepared_roots (c <: U64.t)
 
 let post_roots_mem_a_prime
   (r: unit{ConcreteMajor.spot_major_room})
-  (roots_out: seq U64.t) (st: seq obj_addr)
+  (roots_out: seq U64.t) (st: seq obj_addr) (cap: nat)
   : Lemma
       (requires
         CheneyBFS.cheney_no_oom
@@ -98,7 +118,7 @@ let post_roots_mem_a_prime
           (ConcreteMajor.spot_major_heap r)
           (ConcreteMajor.spot_major_fp r)
           (ThreeObjects.spot_roots (ConcreteMajor.spot_c r))
-          roots_out st)
+          roots_out st cap)
       (ensures (
         let prom = Cheney.cheney_promote
           ConcreteMinor.spot_minor2
@@ -106,7 +126,15 @@ let post_roots_mem_a_prime
           (ConcreteMajor.spot_major_fp r)
           (ThreeObjects.spot_roots (ConcreteMajor.spot_c r)) in
         let img = prom.fwd_map Layout.a_minor in
-        Seq.mem img roots_out /\ is_val_addr img /\ Seq.mem (img <: obj_addr) st)
+        let prepared_roots = GenImpl.gen_gc_prepared_roots
+          ConcreteMinor.spot_minor2
+          (ConcreteMajor.spot_major_heap r)
+          (ConcreteMajor.spot_major_fp r)
+          (ThreeObjects.spot_roots (ConcreteMajor.spot_c r))
+          st cap in
+        Seq.mem img roots_out /\
+        is_val_addr img /\
+        Seq.mem (img <: obj_addr) prepared_roots)
       )
   =
   let c = ConcreteMajor.spot_c r in
@@ -145,23 +173,39 @@ let post_roots_mem_a_prime
   assert (Seq.index roots_out 1 == img);
   FStar.Seq.Properties.seq_mem_k roots_out 1;
   assert (Seq.mem img roots_out);
-  assert (GenImpl.roots_match_stack roots_out st);
-  roots_match_u64_mem_in_stack roots_out st img
+  let prepared_roots = GenImpl.gen_gc_prepared_roots
+    ConcreteMinor.spot_minor2
+    (ConcreteMajor.spot_major_heap r)
+    (ConcreteMajor.spot_major_fp r)
+    roots st cap in
+  assert (GenImpl.roots_match_stack roots_out prepared_roots);
+  roots_match_u64_mem_in_stack roots_out prepared_roots img
 
-let root_heap_reachable_from_stack_shape
-  (major: heap) (st: seq obj_addr) (cap: nat) (r: obj_addr)
+let root_heap_reachable_from_major_gc_pre
+  (minor: minor_state) (major: heap) (fp: U64.t)
+  (roots: seq U64.t) (st: seq obj_addr) (cap: nat) (r: obj_addr)
   : Lemma
-      (requires GenInv.major_stack_shape major st cap /\ Seq.mem r st)
-      (ensures SpecCorrectness.heap_reachable major st r)
+      (requires
+        GenImpl.gen_gc_major_precondition minor major fp roots st cap /\
+        Seq.mem r (GenImpl.gen_gc_prepared_roots minor major fp roots st cap))
+      (ensures
+        SpecCorrectness.heap_reachable
+          (GenImpl.gen_gc_prepared_major minor major fp roots st cap)
+          (GenImpl.gen_gc_prepared_roots minor major fp roots st cap)
+          r)
   =
-  let graph = HeapModel.create_graph major in
-  let roots' = HeapGraph.coerce_to_vertex_list st in
-  GenInv.major_stack_shape_elim major st cap;
-  HeapGraph.coerce_mem_lemma st r;
+  let prepared_major = GenImpl.gen_gc_prepared_major minor major fp roots st cap in
+  let prepared_roots = GenImpl.gen_gc_prepared_roots minor major fp roots st cap in
+  let graph = HeapModel.create_graph prepared_major in
+  let roots' = HeapGraph.coerce_to_vertex_list prepared_roots in
+  assert (MajorGC.gc_precondition_with_roots
+    prepared_major prepared_roots prepared_roots
+    (Cheney.cheney_collect_spec minor major fp roots).mc_fp cap);
+  HeapGraph.coerce_mem_lemma prepared_roots r;
   assert (Seq.mem r roots');
   assert (SpecGraph.mem_graph_vertex graph r);
   assert (Seq.mem r (SpecDFS.reachable_set graph roots'));
-  assert (SpecCorrectness.heap_reachable major st r)
+  assert (SpecCorrectness.heap_reachable prepared_major prepared_roots r)
 
 let spot_concrete_c_final_survives
   (r: unit{ConcreteMajor.spot_major_room})
@@ -182,15 +226,14 @@ let spot_concrete_c_final_survives
           (ConcreteMajor.spot_major_heap r)
           (ConcreteMajor.spot_major_fp r)
           (ThreeObjects.spot_roots (ConcreteMajor.spot_c r))
-          roots_out st /\
-        GenImpl.gen_gc_heap_shape_post
-          d2 b2 result.mc_major final_major result.mc_fp st cap /\
+          roots_out st cap /\
+        GenImpl.gen_gc_heap_shape_post d2 b2 final_major /\
         GenImpl.gen_gc_reachable_subgraph_isomorphism_post
           ConcreteMinor.spot_minor2
           (ConcreteMajor.spot_major_heap r)
           (ConcreteMajor.spot_major_fp r)
           (ThreeObjects.spot_roots (ConcreteMajor.spot_c r))
-          ok final_major roots_out st))
+          ok final_major roots_out st cap))
       (ensures Seq.mem (ConcreteMajor.spot_c r)
         (SpecFields.objects zero_addr final_major))
   =
@@ -201,21 +244,32 @@ let spot_concrete_c_final_survives
       (ConcreteMajor.spot_major_fp r)
       (ThreeObjects.spot_roots (ConcreteMajor.spot_c r)) in
   let c = ConcreteMajor.spot_c r in
-  post_roots_mem_c r roots_out st;
+  post_roots_mem_c r roots_out st cap;
   assert (Seq.mem (c <: U64.t) roots_out);
-  assert (Seq.mem c st);
-  assert (GenInv.full_heap_shape
-    ({ data = d2; bump = b2 } <: minor_state)
-    result.mc_major result.mc_fp st cap);
-  GenInv.full_heap_shape_elim
-    ({ data = d2; bump = b2 } <: minor_state)
-    result.mc_major result.mc_fp st cap;
-  root_heap_reachable_from_stack_shape result.mc_major st cap c;
+  assert (Seq.mem c
+    (GenImpl.gen_gc_prepared_roots
+      ConcreteMinor.spot_minor2
+      (ConcreteMajor.spot_major_heap r)
+      (ConcreteMajor.spot_major_fp r)
+      (ThreeObjects.spot_roots c)
+      st cap));
+  assert (GenImpl.gen_gc_major_precondition
+    ConcreteMinor.spot_minor2
+    (ConcreteMajor.spot_major_heap r)
+    (ConcreteMajor.spot_major_fp r)
+    (ThreeObjects.spot_roots c)
+    st cap);
+  root_heap_reachable_from_major_gc_pre
+    ConcreteMinor.spot_minor2
+    (ConcreteMajor.spot_major_heap r)
+    (ConcreteMajor.spot_major_fp r)
+    (ThreeObjects.spot_roots c)
+    st cap c;
   ThreeObjects.spot_final_survives_from_gen_gc_post
     ConcreteMinor.spot_minor2
     (ConcreteMajor.spot_major_heap r)
     (ConcreteMajor.spot_major_fp r)
-    c roots_out ok final_major st c
+    c roots_out ok final_major st cap c
 
 let spot_concrete_a_prime_final_survives
   (r: unit{ConcreteMajor.spot_major_room})
@@ -231,25 +285,19 @@ let spot_concrete_a_prime_final_survives
             (ConcreteMajor.spot_major_fp r)
             (ThreeObjects.spot_roots (ConcreteMajor.spot_c r)) in
         ok /\
-        CheneyBFS.cheney_no_oom
-          ConcreteMinor.spot_minor2
-          (ConcreteMajor.spot_major_heap r)
-          (ConcreteMajor.spot_major_fp r)
-          (ThreeObjects.spot_roots (ConcreteMajor.spot_c r)) /\
         GenImpl.gen_gc_roots_post
           ConcreteMinor.spot_minor2
           (ConcreteMajor.spot_major_heap r)
           (ConcreteMajor.spot_major_fp r)
           (ThreeObjects.spot_roots (ConcreteMajor.spot_c r))
-          roots_out st /\
-        GenImpl.gen_gc_heap_shape_post
-          d2 b2 result.mc_major final_major result.mc_fp st cap /\
+          roots_out st cap /\
+        GenImpl.gen_gc_heap_shape_post d2 b2 final_major /\
         GenImpl.gen_gc_reachable_subgraph_isomorphism_post
           ConcreteMinor.spot_minor2
           (ConcreteMajor.spot_major_heap r)
           (ConcreteMajor.spot_major_fp r)
           (ThreeObjects.spot_roots (ConcreteMajor.spot_c r))
-          ok final_major roots_out st))
+          ok final_major roots_out st cap))
       (ensures (
         let prom =
           Cheney.cheney_promote
@@ -276,21 +324,33 @@ let spot_concrete_a_prime_final_survives
       (ConcreteMajor.spot_major_fp r)
       (ThreeObjects.spot_roots c) in
   let img = prom.fwd_map Layout.a_minor in
-  post_roots_mem_a_prime r roots_out st;
+  ConcreteForwarding.spot_concrete_no_oom r;
+  post_roots_mem_a_prime r roots_out st cap;
   let a_prime = (img <: obj_addr) in
-  assert (Seq.mem a_prime st);
-  assert (GenInv.full_heap_shape
-    ({ data = d2; bump = b2 } <: minor_state)
-    result.mc_major result.mc_fp st cap);
-  GenInv.full_heap_shape_elim
-    ({ data = d2; bump = b2 } <: minor_state)
-    result.mc_major result.mc_fp st cap;
-  root_heap_reachable_from_stack_shape result.mc_major st cap a_prime;
+  assert (Seq.mem a_prime
+    (GenImpl.gen_gc_prepared_roots
+      ConcreteMinor.spot_minor2
+      (ConcreteMajor.spot_major_heap r)
+      (ConcreteMajor.spot_major_fp r)
+      (ThreeObjects.spot_roots c)
+      st cap));
+  assert (GenImpl.gen_gc_major_precondition
+    ConcreteMinor.spot_minor2
+    (ConcreteMajor.spot_major_heap r)
+    (ConcreteMajor.spot_major_fp r)
+    (ThreeObjects.spot_roots c)
+    st cap);
+  root_heap_reachable_from_major_gc_pre
+    ConcreteMinor.spot_minor2
+    (ConcreteMajor.spot_major_heap r)
+    (ConcreteMajor.spot_major_fp r)
+    (ThreeObjects.spot_roots c)
+    st cap a_prime;
   ThreeObjects.spot_final_survives_from_gen_gc_post
     ConcreteMinor.spot_minor2
     (ConcreteMajor.spot_major_heap r)
     (ConcreteMajor.spot_major_fp r)
-    c roots_out ok final_major st a_prime;
+    c roots_out ok final_major st cap a_prime;
   assert (a_prime == img);
   assert (exists (a_prime: obj_addr).
     a_prime == img /\ Seq.mem a_prime (SpecFields.objects zero_addr final_major))
@@ -365,6 +425,231 @@ let c_field1_get_field
   assert (raw_slot == slot)
 #pop-options
 
+#push-options "--z3rlimit 10 --fuel 0 --ifuel 0"
+let post_roots_shape
+  (r: unit{ConcreteMajor.spot_major_room})
+  (roots_out: seq U64.t) (st: seq obj_addr) (cap: nat)
+  : Lemma
+      (requires
+        CheneyBFS.cheney_no_oom
+          ConcreteMinor.spot_minor2
+          (ConcreteMajor.spot_major_heap r)
+          (ConcreteMajor.spot_major_fp r)
+          (ThreeObjects.spot_roots (ConcreteMajor.spot_c r)) /\
+        GenImpl.gen_gc_roots_post
+          ConcreteMinor.spot_minor2
+          (ConcreteMajor.spot_major_heap r)
+          (ConcreteMajor.spot_major_fp r)
+          (ThreeObjects.spot_roots (ConcreteMajor.spot_c r))
+          roots_out st cap)
+      (ensures (
+        let c = ConcreteMajor.spot_c r in
+        let prom = Cheney.cheney_promote
+          ConcreteMinor.spot_minor2
+          (ConcreteMajor.spot_major_heap r)
+          (ConcreteMajor.spot_major_fp r)
+          (ThreeObjects.spot_roots c) in
+        Seq.length roots_out == 2 /\
+        Seq.index roots_out 0 == (c <: U64.t) /\
+        Seq.index roots_out 1 == prom.fwd_map Layout.a_minor))
+  =
+  let c = ConcreteMajor.spot_c r in
+  let roots = ThreeObjects.spot_roots c in
+  let prom = Cheney.cheney_promote
+    ConcreteMinor.spot_minor2
+    (ConcreteMajor.spot_major_heap r)
+    (ConcreteMajor.spot_major_fp r)
+    roots in
+  let result = Cheney.cheney_collect_spec
+    ConcreteMinor.spot_minor2
+    (ConcreteMajor.spot_major_heap r)
+    (ConcreteMajor.spot_major_fp r)
+    roots in
+  assert (roots_out == result.mc_roots);
+  ThreeObjects.spot_roots_len c;
+  Promote.rewrite_roots_length roots prom.fwd_map;
+  assert (Seq.length roots_out == 2);
+  ThreeObjects.spot_roots_index_c c;
+  Promote.rewrite_roots_index roots prom.fwd_map 0;
+  ConcreteMajor.spot_major_layout_facts r;
+  zero_addr_above_minor ();
+  assert (~(Promote.is_minor_pointer (c <: U64.t)));
+  assert (Promote.rewrite_root (c <: U64.t) prom.fwd_map == (c <: U64.t));
+  assert (Seq.index roots_out 0 == (c <: U64.t));
+  ThreeObjects.spot_roots_index_a c;
+  Promote.rewrite_roots_index roots prom.fwd_map 1;
+  Layout.a_minor_is_minor_pointer ();
+  ConcreteScenarios.spot_concrete_a_promoted_from_no_oom r;
+  Postconditions.promoted_image_elim
+    ConcreteMinor.spot_minor2
+    (ConcreteMajor.spot_major_heap r)
+    (ConcreteMajor.spot_major_fp r)
+    roots Layout.a_minor (prom.fwd_map Layout.a_minor);
+  assert (prom.fwd_map Layout.a_minor <> 0UL);
+  assert (Promote.rewrite_root Layout.a_minor prom.fwd_map ==
+          prom.fwd_map Layout.a_minor);
+  assert (Seq.index roots_out 1 == prom.fwd_map Layout.a_minor)
+
+let nat_lt_two_cases (i: nat)
+  : Lemma (requires i < 2) (ensures i == 0 \/ i == 1)
+  = ()
+
+let object_header_not_c_field1
+  (r: unit{ConcreteMajor.spot_major_room}) (g: heap) (target: obj_addr)
+  : Lemma
+      (requires
+        SpecFields.well_formed_heap g /\
+        Seq.mem (ConcreteMajor.spot_c r) (SpecFields.objects zero_addr g) /\
+        Seq.mem target (SpecFields.objects zero_addr g) /\
+        U64.v (SpecObj.wosize_of_object (ConcreteMajor.spot_c r) g) >= 2)
+      (ensures SpecHeap.hd_address target <> ConcreteMajor.spot_c_field1 r)
+  =
+  let c = ConcreteMajor.spot_c r in
+  let slot = ConcreteMajor.spot_c_field1 r in
+  ConcreteMajor.spot_major_layout_facts r;
+  SpecHeap.hd_address_spec c;
+  SpecHeap.hd_address_spec target;
+  assert (U64.v slot == U64.v c + 8);
+  if target = c then
+    assert (U64.v (SpecHeap.hd_address target) < U64.v slot)
+  else if U64.v target < U64.v c then
+    assert (U64.v (SpecHeap.hd_address target) < U64.v slot)
+  else begin
+    assert (U64.v c < U64.v target);
+    SpecObj.wosize_of_object_bound c g;
+    assert (SpecFields.wosize_of_object_as_wosize c g ==
+            SpecObj.wosize_of_object c g);
+    SpecFields.objects_separated zero_addr g c target;
+    assert (U64.v target > U64.v c + 16);
+    assert (U64.v (SpecHeap.hd_address target) > U64.v slot)
+  end
+
+let prepared_roots_preserve_c_field1
+  (r: unit{ConcreteMajor.spot_major_room})
+  (roots_out: seq U64.t) (st: seq obj_addr) (cap: nat)
+  : Lemma
+      (requires
+        CheneyBFS.cheney_no_oom
+          ConcreteMinor.spot_minor2
+          (ConcreteMajor.spot_major_heap r)
+          (ConcreteMajor.spot_major_fp r)
+          (ThreeObjects.spot_roots (ConcreteMajor.spot_c r)) /\
+        GenImpl.gen_gc_roots_post
+          ConcreteMinor.spot_minor2
+          (ConcreteMajor.spot_major_heap r)
+          (ConcreteMajor.spot_major_fp r)
+          (ThreeObjects.spot_roots (ConcreteMajor.spot_c r))
+          roots_out st cap /\
+        GenImpl.gen_gc_major_precondition
+          ConcreteMinor.spot_minor2
+          (ConcreteMajor.spot_major_heap r)
+          (ConcreteMajor.spot_major_fp r)
+          (ThreeObjects.spot_roots (ConcreteMajor.spot_c r))
+          st cap)
+      (ensures (
+        let result = Cheney.cheney_collect_spec
+          ConcreteMinor.spot_minor2
+          (ConcreteMajor.spot_major_heap r)
+          (ConcreteMajor.spot_major_fp r)
+          (ThreeObjects.spot_roots (ConcreteMajor.spot_c r)) in
+        let prepared_major = GenImpl.gen_gc_prepared_major
+          ConcreteMinor.spot_minor2
+          (ConcreteMajor.spot_major_heap r)
+          (ConcreteMajor.spot_major_fp r)
+          (ThreeObjects.spot_roots (ConcreteMajor.spot_c r))
+          st cap in
+        SpecHeap.read_word prepared_major (ConcreteMajor.spot_c_field1 r) ==
+        SpecHeap.read_word result.mc_major (ConcreteMajor.spot_c_field1 r) /\
+        SpecObj.wosize_of_object (ConcreteMajor.spot_c r) prepared_major ==
+        SpecObj.wosize_of_object (ConcreteMajor.spot_c r) result.mc_major))
+  =
+  let c = ConcreteMajor.spot_c r in
+  let roots = ThreeObjects.spot_roots c in
+  let result = Cheney.cheney_collect_spec
+    ConcreteMinor.spot_minor2
+    (ConcreteMajor.spot_major_heap r)
+    (ConcreteMajor.spot_major_fp r)
+    roots in
+  let prepared_major = GenImpl.gen_gc_prepared_major
+    ConcreteMinor.spot_minor2
+    (ConcreteMajor.spot_major_heap r)
+    (ConcreteMajor.spot_major_fp r)
+    roots st cap in
+  let prepared_roots = GenImpl.gen_gc_prepared_roots
+    ConcreteMinor.spot_minor2
+    (ConcreteMajor.spot_major_heap r)
+    (ConcreteMajor.spot_major_fp r)
+    roots st cap in
+  post_roots_shape r roots_out st cap;
+  post_roots_mem_c r roots_out st cap;
+  post_roots_mem_a_prime r roots_out st cap;
+  post_minor_c_wosize r;
+  assert (roots_out == result.mc_roots);
+  assert (prepared_major ==
+          fst (MarkBoundedImpl.darken_roots_bounded_spec
+            result.mc_major st roots_out cap));
+  MarkBoundedImpl.darken_roots_bounded_spec_preserves_wosize
+    result.mc_major st roots_out cap c;
+  assert (SpecObj.wosize_of_object c prepared_major ==
+          SpecObj.wosize_of_object c result.mc_major);
+  assert (U64.v (SpecObj.wosize_of_object c prepared_major) >= 2);
+  assert (MajorGC.gc_precondition_with_roots
+    prepared_major prepared_roots prepared_roots result.mc_fp cap);
+  assert (SpecMarkBoundedInv.bounded_mark_inv prepared_major prepared_roots cap);
+  SpecMarkBoundedInv.bounded_mark_inv_elim_wfh prepared_major prepared_roots cap;
+  assert (SpecMark.root_props prepared_major prepared_roots);
+  assert (Seq.mem c prepared_roots);
+  assert (Seq.mem c (SpecFields.objects zero_addr prepared_major));
+  let prom = Cheney.cheney_promote
+    ConcreteMinor.spot_minor2
+    (ConcreteMajor.spot_major_heap r)
+    (ConcreteMajor.spot_major_fp r)
+    roots in
+  let img = prom.fwd_map Layout.a_minor in
+  let a_prime = (img <: obj_addr) in
+  assert (Seq.mem a_prime prepared_roots);
+  assert (Seq.mem a_prime (SpecFields.objects zero_addr prepared_major));
+  let slot = ConcreteMajor.spot_c_field1 r in
+  let no_root_header (i: nat)
+    : Lemma
+        (ensures
+          i < Seq.length roots_out ==>
+          (U64.v (Seq.index roots_out i) >= U64.v zero_addr + U64.v mword /\
+           U64.v (Seq.index roots_out i) < heap_size /\
+           U64.v (Seq.index roots_out i) % U64.v mword == 0 ==>
+           U64.sub (Seq.index roots_out i) mword <> slot))
+    =
+    if i < Seq.length roots_out then begin
+      assert (Seq.length roots_out == 2);
+      match i with
+      | 0 ->
+        assert (Seq.index roots_out i == (c <: U64.t));
+        object_header_not_c_field1 r prepared_major c;
+        SpecHeap.hd_address_spec c;
+        assert (U64.v (U64.sub (Seq.index roots_out i) mword) ==
+                U64.v (SpecHeap.hd_address c));
+        U64.v_inj (U64.sub (Seq.index roots_out i) mword) (SpecHeap.hd_address c);
+        assert (U64.sub (Seq.index roots_out i) mword == SpecHeap.hd_address c)
+      | 1 ->
+        assert (Seq.index roots_out i == img);
+        object_header_not_c_field1 r prepared_major a_prime;
+        assert (Seq.index roots_out i == (a_prime <: U64.t));
+        SpecHeap.hd_address_spec a_prime;
+        assert (U64.v (U64.sub (Seq.index roots_out i) mword) ==
+                U64.v (SpecHeap.hd_address a_prime));
+        U64.v_inj (U64.sub (Seq.index roots_out i) mword) (SpecHeap.hd_address a_prime);
+        assert (U64.sub (Seq.index roots_out i) mword ==
+                SpecHeap.hd_address a_prime)
+      | _ ->
+        nat_lt_two_cases i;
+        assert False
+    end
+  in
+  FStar.Classical.forall_intro no_root_header;
+  MarkBoundedImpl.darken_roots_bounded_spec_preserves_read_word
+    result.mc_major st roots_out cap slot
+#pop-options
+
 let spot_concrete_c_field_final_points_to_a_prime
   (r: unit{ConcreteMajor.spot_major_room})
   (d2: minor_heap) (b2: U64.t)
@@ -379,25 +664,19 @@ let spot_concrete_c_field_final_points_to_a_prime
             (ConcreteMajor.spot_major_fp r)
             (ThreeObjects.spot_roots (ConcreteMajor.spot_c r)) in
         ok /\
-        CheneyBFS.cheney_no_oom
-          ConcreteMinor.spot_minor2
-          (ConcreteMajor.spot_major_heap r)
-          (ConcreteMajor.spot_major_fp r)
-          (ThreeObjects.spot_roots (ConcreteMajor.spot_c r)) /\
         GenImpl.gen_gc_roots_post
           ConcreteMinor.spot_minor2
           (ConcreteMajor.spot_major_heap r)
           (ConcreteMajor.spot_major_fp r)
           (ThreeObjects.spot_roots (ConcreteMajor.spot_c r))
-          roots_out st /\
-        GenImpl.gen_gc_heap_shape_post
-          d2 b2 result.mc_major final_major result.mc_fp st cap /\
+          roots_out st cap /\
+        GenImpl.gen_gc_heap_shape_post d2 b2 final_major /\
         GenImpl.gen_gc_reachable_subgraph_isomorphism_post
           ConcreteMinor.spot_minor2
           (ConcreteMajor.spot_major_heap r)
           (ConcreteMajor.spot_major_fp r)
           (ThreeObjects.spot_roots (ConcreteMajor.spot_c r))
-          ok final_major roots_out st))
+          ok final_major roots_out st cap))
       (ensures (
         let prom =
           Cheney.cheney_promote
@@ -427,31 +706,59 @@ let spot_concrete_c_field_final_points_to_a_prime
       (ConcreteMajor.spot_major_fp r)
       (ThreeObjects.spot_roots c) in
   let img = prom.fwd_map Layout.a_minor in
+  ConcreteForwarding.spot_concrete_no_oom r;
   ConcreteScenarios.spot_concrete_c_field_rewritten_from_no_oom r;
   post_minor_c_wosize r;
-  post_roots_mem_c r roots_out st;
-  post_roots_mem_a_prime r roots_out st;
+  post_roots_mem_c r roots_out st cap;
+  post_roots_mem_a_prime r roots_out st cap;
   let a_prime = (img <: obj_addr) in
-  assert (Seq.mem c st);
-  assert (Seq.mem a_prime st);
-  assert (GenInv.full_heap_shape
-    ({ data = d2; bump = b2 } <: minor_state)
-    result.mc_major result.mc_fp st cap);
-  GenInv.full_heap_shape_elim
-    ({ data = d2; bump = b2 } <: minor_state)
-    result.mc_major result.mc_fp st cap;
-  root_heap_reachable_from_stack_shape result.mc_major st cap c;
-  root_heap_reachable_from_stack_shape result.mc_major st cap a_prime;
+  let prepared_major = GenImpl.gen_gc_prepared_major
+    ConcreteMinor.spot_minor2
+    (ConcreteMajor.spot_major_heap r)
+    (ConcreteMajor.spot_major_fp r)
+    (ThreeObjects.spot_roots c)
+    st cap in
+  let prepared_roots = GenImpl.gen_gc_prepared_roots
+    ConcreteMinor.spot_minor2
+    (ConcreteMajor.spot_major_heap r)
+    (ConcreteMajor.spot_major_fp r)
+    (ThreeObjects.spot_roots c)
+    st cap in
+  assert (Seq.mem c prepared_roots);
+  assert (Seq.mem a_prime prepared_roots);
+  assert (GenImpl.gen_gc_major_precondition
+    ConcreteMinor.spot_minor2
+    (ConcreteMajor.spot_major_heap r)
+    (ConcreteMajor.spot_major_fp r)
+    (ThreeObjects.spot_roots c)
+    st cap);
+  root_heap_reachable_from_major_gc_pre
+    ConcreteMinor.spot_minor2
+    (ConcreteMajor.spot_major_heap r)
+    (ConcreteMajor.spot_major_fp r)
+    (ThreeObjects.spot_roots c)
+    st cap c;
+  root_heap_reachable_from_major_gc_pre
+    ConcreteMinor.spot_minor2
+    (ConcreteMajor.spot_major_heap r)
+    (ConcreteMajor.spot_major_fp r)
+    (ThreeObjects.spot_roots c)
+    st cap a_prime;
   assert (SpecCorrectness.major_gc_live_subgraph_isomorphism
-    result.mc_major final_major st);
-  c_field1_get_field r result.mc_major;
+    prepared_major final_major prepared_roots);
+  prepared_roots_preserve_c_field1 r roots_out st cap;
+  c_field1_get_field r prepared_major;
   c_field1_get_field r final_major;
-  assert (U64.v 2UL <= U64.v (SpecObj.wosize_of_object c result.mc_major));
-  assert (HeapGraph.get_field result.mc_major c 2UL ==
+  assert (U64.v 2UL <= U64.v (SpecObj.wosize_of_object c prepared_major));
+  assert (HeapGraph.get_field prepared_major c 2UL ==
           HeapGraph.get_field final_major c 2UL);
   spot_concrete_c_final_survives r d2 b2 roots_out ok final_major st cap;
   spot_concrete_a_prime_final_survives r d2 b2 roots_out ok final_major st cap;
   assert (SpecHeap.read_word result.mc_major (ConcreteMajor.spot_c_field1 r) ==
+          img);
+  assert (SpecHeap.read_word prepared_major (ConcreteMajor.spot_c_field1 r) ==
+          SpecHeap.read_word result.mc_major (ConcreteMajor.spot_c_field1 r));
+  assert (SpecHeap.read_word prepared_major (ConcreteMajor.spot_c_field1 r) ==
           img);
   assert (SpecHeap.read_word final_major (ConcreteMajor.spot_c_field1 r) ==
           img);
