spot/GC.SPOT.ConcreteFull.fsti
@@ -33,15 +33,14 @@ val spot_concrete_c_final_survives
           (ConcreteMajor.spot_major_heap r)
           (ConcreteMajor.spot_major_fp r)
           (ThreeObjects.spot_roots (ConcreteMajor.spot_c r))
-          roots_out st /\
-        GenImpl.gen_gc_heap_shape_post
-          d2 b2 result.mc_major final_major result.mc_fp st cap /\
+          roots_out st cap /\
+        GenImpl.gen_gc_heap_shape_post d2 b2 final_major /\
         GenImpl.gen_gc_reachable_subgraph_isomorphism_post
           ConcreteMinor.spot_minor2
           (ConcreteMajor.spot_major_heap r)
           (ConcreteMajor.spot_major_fp r)
           (ThreeObjects.spot_roots (ConcreteMajor.spot_c r))
-          ok final_major roots_out st))
+          ok final_major roots_out st cap))
       (ensures Seq.mem (ConcreteMajor.spot_c r)
         (GC.Spec.Fields.objects zero_addr final_major))
 
@@ -59,25 +58,19 @@ val spot_concrete_a_prime_final_survives
             (ConcreteMajor.spot_major_fp r)
             (ThreeObjects.spot_roots (ConcreteMajor.spot_c r)) in
         ok /\
-        GC.Gen.CheneyBFS.cheney_no_oom
-          ConcreteMinor.spot_minor2
-          (ConcreteMajor.spot_major_heap r)
-          (ConcreteMajor.spot_major_fp r)
-          (ThreeObjects.spot_roots (ConcreteMajor.spot_c r)) /\
         GenImpl.gen_gc_roots_post
           ConcreteMinor.spot_minor2
           (ConcreteMajor.spot_major_heap r)
           (ConcreteMajor.spot_major_fp r)
           (ThreeObjects.spot_roots (ConcreteMajor.spot_c r))
-          roots_out st /\
-        GenImpl.gen_gc_heap_shape_post
-          d2 b2 result.mc_major final_major result.mc_fp st cap /\
+          roots_out st cap /\
+        GenImpl.gen_gc_heap_shape_post d2 b2 final_major /\
         GenImpl.gen_gc_reachable_subgraph_isomorphism_post
           ConcreteMinor.spot_minor2
           (ConcreteMajor.spot_major_heap r)
           (ConcreteMajor.spot_major_fp r)
           (ThreeObjects.spot_roots (ConcreteMajor.spot_c r))
-          ok final_major roots_out st))
+          ok final_major roots_out st cap))
       (ensures (
         let prom =
           Cheney.cheney_promote
@@ -104,25 +97,19 @@ val spot_concrete_c_field_final_points_to_a_prime
             (ConcreteMajor.spot_major_fp r)
             (ThreeObjects.spot_roots (ConcreteMajor.spot_c r)) in
         ok /\
-        GC.Gen.CheneyBFS.cheney_no_oom
-          ConcreteMinor.spot_minor2
-          (ConcreteMajor.spot_major_heap r)
-          (ConcreteMajor.spot_major_fp r)
-          (ThreeObjects.spot_roots (ConcreteMajor.spot_c r)) /\
         GenImpl.gen_gc_roots_post
           ConcreteMinor.spot_minor2
           (ConcreteMajor.spot_major_heap r)
           (ConcreteMajor.spot_major_fp r)
           (ThreeObjects.spot_roots (ConcreteMajor.spot_c r))
-          roots_out st /\
-        GenImpl.gen_gc_heap_shape_post
-          d2 b2 result.mc_major final_major result.mc_fp st cap /\
+          roots_out st cap /\
+        GenImpl.gen_gc_heap_shape_post d2 b2 final_major /\
         GenImpl.gen_gc_reachable_subgraph_isomorphism_post
           ConcreteMinor.spot_minor2
           (ConcreteMajor.spot_major_heap r)
           (ConcreteMajor.spot_major_fp r)
           (ThreeObjects.spot_roots (ConcreteMajor.spot_c r))
-          ok final_major roots_out st))
+          ok final_major roots_out st cap))
       (ensures (
         let prom =
           Cheney.cheney_promote
